src/tactics/FStarC.Tactics.Interpreter.fst
@@ -56,6 +56,9 @@ module U       = FStarC.Syntax.Util
 
 let dbg_Tac = Debug.get_toggle "Tac"
 
+(* Inlined for extraction: see the note on the copy in
+   FStarC.TypeChecker.Primops.Base. *)
+inline_for_extraction
 let solve (#a:Type) {| ev : a |} : Tot a = ev
 
 let embed {|embedding 'a|} r (x:'a) norm_cb = embed x r None norm_cb
